<?xml version="1.0" encoding="UTF-8"?>

<!DOCTYPE rdf:RDF [
  <!ENTITY sed  "http://sweet.jpl.nasa.gov/2.3/matrSediment.owl">
  <!ENTITY comp "http://sweet.jpl.nasa.gov/2.3/matrCompound.owl">
  <!ENTITY orog "http://sweet.jpl.nasa.gov/2.3/realmLandOrographic.owl">
  <!ENTITY meso "http://sweet.jpl.nasa.gov/2.3/phenAtmoWindMesoscale.owl">
  <!ENTITY statec "http://sweet.jpl.nasa.gov/2.3/procStateChange.owl">
  <!ENTITY water "http://sweet.jpl.nasa.gov/2.3/matrWater.owl">
  <!ENTITY mix "http://sweet.jpl.nasa.gov/2.3/phenMixing.owl">
  <!ENTITY cloud "http://sweet.jpl.nasa.gov/2.3/phenAtmoCloud.owl">
  <!ENTITY coast "http://sweet.jpl.nasa.gov/2.3/realmLandCoastal.owl">
  <!ENTITY fog "http://sweet.jpl.nasa.gov/2.3/phenAtmoFog.owl">
  <!ENTITY srela "http://sweet.jpl.nasa.gov/2.3/relaSpace.owl">
  <!ENTITY crela "http://sweet.jpl.nasa.gov/2.3/relaChemical.owl">
  <!ENTITY prela "http://sweet.jpl.nasa.gov/2.3/relaPhysical.owl">
  <!ENTITY rela "http://sweet.jpl.nasa.gov/2.3/rela.owl">
  <!ENTITY trans "http://sweet.jpl.nasa.gov/2.3/phenFluidTransport.owl">
  <!ENTITY front "http://sweet.jpl.nasa.gov/2.3/phenAtmoFront.owl">
  <!ENTITY planet "http://sweet.jpl.nasa.gov/2.3/realm.owl">
  <!ENTITY phen "http://sweet.jpl.nasa.gov/2.3/phen.owl">
  <!ENTITY precip "http://sweet.jpl.nasa.gov/2.3/phenAtmoPrecipitation.owl">
  <!ENTITY owl "http://www.w3.org/2002/07/owl#">
  <!ENTITY rdf "http://www.w3.org/1999/02/22-rdf-syntax-ns#">
  <!ENTITY rdfs "http://www.w3.org/2000/01/rdf-schema#">
  <!ENTITY xsd "http://www.w3.org/2001/XMLSchema#">
]>

<rdf:RDF xml:base="&fog;"
         xmlns:fog="&fog;"
         xmlns:sed="&sed;"
         xmlns:orog="&orog;"
         xmlns:comp="&comp;"
         xmlns:meso="&meso;"
         xmlns:srela="&srela;"
         xmlns:crela="&crela;"
         xmlns:prela="&prela;"
         xmlns:rela="&rela;"
         xmlns:statec="&statec;"
         xmlns:coast="&coast;"
         xmlns:water="&water;"
         xmlns:cloud="&cloud;"
         xmlns:mix="&mix;"
         xmlns:planet="&planet;"
         xmlns:phen="&phen;"
         xmlns:precip="&precip;"
         xmlns:front="&front;"
         xmlns:trans="&trans;"
         xmlns:owl="&owl;"
         xmlns:rdf="&rdf;"
         xmlns:rdfs="&rdfs;"
 	 xmlns:xsd="&xsd;">

<!-- Ontology Information -->
<!-- Ontology Information -->
  <owl:Ontology rdf:about="" owl:versionInfo="2.3">
     <rdfs:label>SWEET Ontology</rdfs:label>
     <owl:imports rdf:resource="&sed;"/>
     <owl:imports rdf:resource="&meso;"/>
     <owl:imports rdf:resource="&statec;"/>
     <owl:imports rdf:resource="&water;"/>
     <owl:imports rdf:resource="&cloud;"/>
     <owl:imports rdf:resource="&coast;"/>
     <owl:imports rdf:resource="&srela;"/>
     <owl:imports rdf:resource="&crela;"/>
     <owl:imports rdf:resource="&prela;"/>
     <owl:imports rdf:resource="&rela;"/>
     <owl:imports rdf:resource="&comp;"/>
     <owl:imports rdf:resource="&planet;"/>
     <owl:imports rdf:resource="&phen;"/>
     <owl:imports rdf:resource="&precip;"/>
     <owl:imports rdf:resource="&mix;"/>
     <owl:imports rdf:resource="&trans;"/>
     <owl:imports rdf:resource="&front;"/>
     <owl:imports rdf:resource="&orog;"/>
  </owl:Ontology>

<!-- Phenomena -->
  <owl:Class rdf:about="#advectionfog">
    <rdfs:subClassOf rdf:resource="#fog" />
    <rdfs:subClassOf>
      <owl:Restriction>
        <owl:onProperty rdf:resource="&rela;#hasphenomena" />
        <owl:allValuesFrom rdf:resource="&trans;#advection" />
      </owl:Restriction>
    </rdfs:subClassOf>
    <rdfs:label>AdvectionFog</rdfs:label>
    <rdfs:comment>A type of fog caused by the advection of moist air over a cold surface, and the consequent cooling of that air to below its dewpoint.
    </rdfs:comment>
  </owl:Class>

  <owl:Class rdf:about="#evaporationfog">
    <rdfs:subClassOf rdf:resource="#fog" />
    <rdfs:subClassOf>
      <owl:Restriction>
        <owl:onProperty rdf:resource="&prela;#hasstatechang" />
        <owl:allValuesFrom rdf:resource="&statec;#evapor" />
      </owl:Restriction>
    </rdfs:subClassOf>
    <rdfs:comment xml:lang="en">Fog formed as a result of evaporation of water that is warmer than the air.</rdfs:comment>
  </owl:Class>

  <owl:Class rdf:about="#fog">
    <rdfs:subClassOf rdf:resource="&cloud;#stratiform"/>
    <rdfs:subClassOf>
      <owl:Restriction>
        <owl:allValuesFrom rdf:resource="&planet;#planetarysurfac"/>
        <owl:onProperty rdf:resource="&rela;#hasrealm"/>
      </owl:Restriction>
    </rdfs:subClassOf>
    <rdfs:comment xml:lang="en">Water droplets suspended in the atmosphere in the vicinity the earth's surface that affect visibility.</rdfs:comment>
    </owl:Class>

 <owl:Class rdf:about="#freezingfog">
    <rdfs:subClassOf rdf:resource="#fog" />
    <rdfs:subClassOf>
      <owl:Restriction>
        <owl:onProperty rdf:resource="&prela;#hasstatechang" />
        <owl:allValuesFrom rdf:resource="&statec;#freez" />
      </owl:Restriction>
    </rdfs:subClassOf>
    <rdfs:comment xml:lang="en">A fog the droplets of which freeze upon contact with exposed objects and form a coating of rime and/or glaze.</rdfs:comment>
  </owl:Class>

  <owl:Class rdf:about="#frontalfog">
    <rdfs:subClassOf>
      <owl:Restriction>
        <owl:onProperty rdf:resource="&rela;#hasphenomena" />
        <owl:allValuesFrom rdf:resource="&front;#front" />
      </owl:Restriction>
    </rdfs:subClassOf>
    <rdfs:subClassOf rdf:resource="#fog" />
    <rdfs:comment xml:lang="en">Fog associated with frontal zones and frontal passages. It is usually divided into three types: warm-front prefrontal fog; cold-front post-frontal fog; and frontal-passage fog. The first two types are a result of rain falling into cold stable air and raising the dewpoint temperature. Frontal-passage fog can result from the ?mixing of warm and cold air masses in the frontal zone? or by ?sudden cooling of air over moist ground.?</rdfs:comment>
  </owl:Class>

  <owl:Class rdf:about="#garua">
    <rdfs:subClassOf rdf:resource="#fog" />
    <rdfs:comment xml:lang="en">A dense fog and/or drizzle from low stratus on the west coast of South America. It creates a raw, cold atmosphere that may last for weeks in winter and supplies a limited amount of moisture to the area.</rdfs:comment>
  </owl:Class>

  <owl:Class rdf:about="#groundfog">
    <rdfs:subClassOf rdf:resource="#fog" />
    <rdfs:subClassOf>
      <owl:Restriction>
        <owl:onProperty rdf:resource="&srela;#near" />
        <owl:allValuesFrom rdf:resource="&planet;#planetarysurfac" />
      </owl:Restriction>
    </rdfs:subClassOf>
    <rdfs:comment xml:lang="en">1. According to U.S. weather observing practice, a fog that hides less than 0.6 of the sky and does not extend to the base of any clouds that may lie above it. As an obstruction to vision in an aviation weather observation, ground fog is encoded GF. 2. See radiation fog.</rdfs:comment>
  </owl:Class>

  <owl:Class rdf:about="#haar">
    <rdfs:subClassOf rdf:resource="#fog" />
    <rdfs:subClassOf>
      <owl:Restriction>
        <owl:onProperty rdf:resource="&rela;#hasrealm" />
        <owl:allValuesFrom rdf:resource="&coast;#coastal" />
      </owl:Restriction>
    </rdfs:subClassOf>
    <rdfs:comment xml:lang="en">A name applied to a wet sea fog or very fine drizzle that drifts in from the sea in coastal districts of eastern Scotland and northeastern England. It occurs most frequently in summer.</rdfs:comment>
  </owl:Class>

  <owl:Class rdf:about="#highfog">
    <rdfs:subClassOf rdf:resource="#mountainfog" />
    <rdfs:comment xml:lang="en">In the US, the frequent fog on the slopes of the coastal mountains of California, especially applied when the fog overtops the range and extends as stratus over the leeward valleys.</rdfs:comment>
  </owl:Class>

 <owl:Class rdf:about="#icefog">
    <rdfs:subClassOf rdf:resource="#fog" />
    <rdfs:subClassOf>
      <owl:Restriction>
        <owl:onProperty rdf:resource="&crela;#hassubst" />
        <owl:allValuesFrom rdf:resource="&water;#ice" />
      </owl:Restriction>
    </rdfs:subClassOf>
    <rdfs:comment xml:lang="en">A type of fog, composed of suspended particles of ice, partly ice crystals 20 to 100 m in diameter, but chiefly, especially when dense, droxtals 12?20 m in diameter. It occurs at very low temperatures, and usually in clear, calm weather in high latitudes. The sun is usually visible and may cause halo phenomena. Ice fog is rare at temperatures warmer than -30?C, and increases in frequency with decreasing temperature until it is almost always present at air temperatures of -45?C in the vicinity of a source of water vapor. Such sources are the open water of fast-flowing streams or of the sea, herds of animals, volcanoes, and especially products of combustion for heating or propulsion. At temperatures warmer than -30?C, these sources can cause steam fog of liquid water droplets, which may turn into ice fog when cooled (see frost smoke). See ice-crystal haze, arctic mist.</rdfs:comment>
  </owl:Class>

  <owl:Class rdf:about="#mixingfog">
    <rdfs:subClassOf rdf:resource="#fog" />
    <rdfs:subClassOf>
      <owl:Restriction>
        <owl:onProperty rdf:resource="&rela;#hasphenomena" />
        <owl:someValuesFrom rdf:resource="&mix;#mix" />
      </owl:Restriction>
    </rdfs:subClassOf>
    <rdfs:comment xml:lang="en">Fog, light and of short duration, produced by the mixing of two moist but nonsaturated air masses with different temperatures.</rdfs:comment>
  </owl:Class>

  <owl:Class rdf:about="#monsoonfog">
    <rdfs:subClassOf rdf:resource="#fog" />
    <rdfs:subClassOf>
      <owl:Restriction>
        <owl:onProperty rdf:resource="&rela;#hasphenomena" />
        <owl:allValuesFrom rdf:resource="&precip;#monsoon" />
      </owl:Restriction>
    </rdfs:subClassOf>
    <rdfs:subClassOf>
      <owl:Restriction>
        <owl:onProperty rdf:resource="&rela;#hasphenomena" />
        <owl:allValuesFrom rdf:resource="&trans;#advection" />
      </owl:Restriction>
    </rdfs:subClassOf>
    <rdfs:comment xml:lang="en">An advection fog produced as a monsoon circulation that transports warm moist air over a colder surface.</rdfs:comment>
  </owl:Class>

  <owl:Class rdf:about="#mountainfog">
    <rdfs:subClassOf rdf:resource="#fog" />
    <owl:equivalentClass rdf:resource="#orographicfog" />
    <rdfs:subClassOf>
      <owl:Restriction>
        <owl:onProperty rdf:resource="&rela;#hasrealm" />
        <owl:someValuesFrom rdf:resource="&orog;#mountain" />
      </owl:Restriction>
    </rdfs:subClassOf>
    <rdfs:comment xml:lang="en">Fog formed by orographic lifting to condensation of moist air up a mountain slope.
    </rdfs:comment>
  </owl:Class>
  <owl:Class rdf:about="#orographicfog"/>

  <owl:Class rdf:about="#radiationfog">
    <rdfs:subClassOf rdf:resource="#fog" />
    <rdfs:subClassOf>
      <owl:Restriction>
        <owl:onProperty rdf:resource="&rela;#hasphenomena" />
        <owl:allValuesFrom rdf:resource="&phen;#radiationalcool" />
      </owl:Restriction>
    </rdfs:subClassOf>
    <rdfs:subClassOf>
      <owl:Restriction>
        <owl:onProperty rdf:resource="&rela;#hasrealm" />
        <owl:allValuesFrom rdf:resource="&planet;#land" />
      </owl:Restriction>
    </rdfs:subClassOf>
    <rdfs:comment xml:lang="en">A common type of fog, produced over a land area when radiational cooling reduces the air temperature to or below its dewpoint.</rdfs:comment>
  </owl:Class>

  <owl:Class rdf:about="#upslopefog">
    <rdfs:subClassOf rdf:resource="#fog" />
    <rdfs:subClassOf>
      <owl:Restriction>
        <owl:onProperty rdf:resource="&rela;#hasphenomena" />
        <owl:allValuesFrom rdf:resource="&meso;#upslopewind" />
      </owl:Restriction>
    </rdfs:subClassOf>
    <rdfs:comment xml:lang="en">A type of fog formed when air flows upward over rising terrain and is, consequently, adiabatically cooled to or below its dewpoint.</rdfs:comment>
  </owl:Class>

  <owl:Class rdf:about="#salthaz">
    <rdfs:subClassOf rdf:resource="#haze" />
    <rdfs:subClassOf>
      <owl:Restriction>
        <owl:onProperty rdf:resource="&crela;#hassubst" />
        <owl:hasValue rdf:resource="&comp;#salt" />
      </owl:Restriction>
    </rdfs:subClassOf>
    <rdfs:comment xml:lang="en">A haze created by the presence of finely divided particles of sea salt in the air, usually derived from the evaporation of sea spray.</rdfs:comment>
  </owl:Class>

  <owl:Class rdf:about="#haze">
    <rdfs:subClassOf rdf:resource="#fog"/>
    <rdfs:comment xml:lang="en">Particles suspended, reducing visibility by scattering light; often a mixture of aerosols and photochemical smog.</rdfs:comment>
  </owl:Class>

  <owl:Class rdf:about="#sandhaz">
    <rdfs:subClassOf rdf:resource="#haze" />
    <rdfs:subClassOf>
      <owl:Restriction>
        <owl:onProperty rdf:resource="&crela;#hassubst" />
        <owl:someValuesFrom rdf:resource="&sed;#sand" />
      </owl:Restriction>
    </rdfs:subClassOf>
    <rdfs:comment xml:lang="en">Reduced visibility in the atmospheric boundary layer caused by suspended particles of soil, mixed into the air during strong winds.</rdfs:comment>
  </owl:Class>

  <owl:Class rdf:about="#smog">
    <rdfs:subClassOf rdf:resource="#fog" />
    <rdfs:comment xml:lang="en">A natural fog contaminated by industrial pollutants, a mixture of smoke and fog.
    </rdfs:comment>
  </owl:Class>

  <owl:Class rdf:about="#browncloud">
    <rdfs:subClassOf rdf:resource="#smog" />
    <rdfs:comment xml:lang="en">Phenomenon particularly associated with smog episodes in cities such as Denver, Colorado. </rdfs:comment>
  </owl:Class>

</rdf:RDF>
